lean4/Automaton/Regex/Zero.lean
@@ -10,14 +10,16 @@ variable {σ : Type _} (q₁ q₂ : Type _) {σs : Finset σ}  [DecidableEq q₁
 
 def zeroNfa : NFA σs := {q := Nat, qs := {}, q₀ := {}, fs := {}, δ := fun _ _ => {}}
 
-theorem not_accepts (w : word σs) : ¬nfa_accepts zeroNfa w := by
-  intro acc
-  simp only [nfa_accepts,zeroNfa,δ_star] at acc
-  rw [δ_star'_empty,Finset.Nonempty] at acc
-  apply Exists.elim acc
-  intro x xin
-  rw [Finset.mem_inter] at xin
-  apply Finset.not_mem_empty
-  apply xin.1
+theorem accepts_iff (w : word σs) : nfa_accepts zeroNfa w ↔ False := by
+  apply Iff.intro
+  · intro na
+    simp only [zeroNfa,nfa_accepts,Finset.Nonempty] at na
+    apply Exists.elim na
+    intro x xin
+    rw [Finset.mem_inter] at xin
+    apply Finset.not_mem_empty
+    exact xin.2
+  · intro f
+    trivial
 
 end Zero
